pulse/src/ocaml/plugin/generated/Pulse_Checker_WithLocalArray.ml
@@ -3,26 +3,23 @@ let (extend_post_hint :
   Pulse_Typing_Env.env ->
     unit Pulse_Typing.post_hint_for_env ->
       Pulse_Syntax_Base.term ->
-        Pulse_Syntax_Base.term ->
-          Pulse_Syntax_Base.var -> unit Pulse_Typing.post_hint_for_env)
+        Pulse_Syntax_Base.var -> unit Pulse_Typing.post_hint_for_env)
   =
   fun g ->
     fun p ->
       fun init_t ->
-        fun len ->
-          fun x ->
-            {
-              Pulse_Typing.g = (p.Pulse_Typing.g);
-              Pulse_Typing.ctag_hint = (p.Pulse_Typing.ctag_hint);
-              Pulse_Typing.ret_ty = (p.Pulse_Typing.ret_ty);
-              Pulse_Typing.u = (p.Pulse_Typing.u);
-              Pulse_Typing.ty_typing = ();
-              Pulse_Typing.post =
-                (Pulse_Typing.comp_withlocal_array_body_post
-                   p.Pulse_Typing.post init_t (Pulse_Syntax_Pure.null_var x)
-                   len);
-              Pulse_Typing.post_typing = ()
-            }
+        fun x ->
+          {
+            Pulse_Typing.g = (p.Pulse_Typing.g);
+            Pulse_Typing.ctag_hint = (p.Pulse_Typing.ctag_hint);
+            Pulse_Typing.ret_ty = (p.Pulse_Typing.ret_ty);
+            Pulse_Typing.u = (p.Pulse_Typing.u);
+            Pulse_Typing.ty_typing = ();
+            Pulse_Typing.post =
+              (Pulse_Typing.comp_withlocal_array_body_post
+                 p.Pulse_Typing.post init_t (Pulse_Syntax_Pure.null_var x));
+            Pulse_Typing.post_typing = ()
+          }
 
 let (is_annotated_type_array :
   Pulse_Syntax_Base.term ->
@@ -61,14 +58,14 @@ let (check :
                      (Obj.magic
                         (FStar_Range.mk_range
                            "Pulse.Checker.WithLocalArray.fst"
-                           (Prims.of_int (59)) (Prims.of_int (10))
-                           (Prims.of_int (59)) (Prims.of_int (56)))))
+                           (Prims.of_int (58)) (Prims.of_int (10))
+                           (Prims.of_int (58)) (Prims.of_int (56)))))
                   (FStar_Sealed.seal
                      (Obj.magic
                         (FStar_Range.mk_range
                            "Pulse.Checker.WithLocalArray.fst"
-                           (Prims.of_int (59)) (Prims.of_int (59))
-                           (Prims.of_int (140)) (Prims.of_int (38)))))
+                           (Prims.of_int (58)) (Prims.of_int (59))
+                           (Prims.of_int (139)) (Prims.of_int (38)))))
                   (FStar_Tactics_Effect.lift_div_tac
                      (fun uu___ ->
                         Pulse_Checker_Pure.push_context
@@ -82,14 +79,14 @@ let (check :
                                 (Obj.magic
                                    (FStar_Range.mk_range
                                       "Pulse.Checker.WithLocalArray.fst"
-                                      (Prims.of_int (60)) (Prims.of_int (62))
-                                      (Prims.of_int (60)) (Prims.of_int (68)))))
+                                      (Prims.of_int (59)) (Prims.of_int (62))
+                                      (Prims.of_int (59)) (Prims.of_int (68)))))
                              (FStar_Sealed.seal
                                 (Obj.magic
                                    (FStar_Range.mk_range
                                       "Pulse.Checker.WithLocalArray.fst"
-                                      (Prims.of_int (59)) (Prims.of_int (59))
-                                      (Prims.of_int (140))
+                                      (Prims.of_int (58)) (Prims.of_int (59))
+                                      (Prims.of_int (139))
                                       (Prims.of_int (38)))))
                              (FStar_Tactics_Effect.lift_div_tac
                                 (fun uu___ -> t.Pulse_Syntax_Base.term1))
@@ -109,17 +106,17 @@ let (check :
                                                (Obj.magic
                                                   (FStar_Range.mk_range
                                                      "Pulse.Checker.WithLocalArray.fst"
-                                                     (Prims.of_int (61))
+                                                     (Prims.of_int (60))
                                                      (Prims.of_int (62))
-                                                     (Prims.of_int (79))
+                                                     (Prims.of_int (78))
                                                      (Prims.of_int (83)))))
                                             (FStar_Sealed.seal
                                                (Obj.magic
                                                   (FStar_Range.mk_range
                                                      "Pulse.Checker.WithLocalArray.fst"
-                                                     (Prims.of_int (60))
+                                                     (Prims.of_int (59))
                                                      (Prims.of_int (71))
-                                                     (Prims.of_int (140))
+                                                     (Prims.of_int (139))
                                                      (Prims.of_int (38)))))
                                             (Obj.magic
                                                (FStar_Tactics_Effect.tac_bind
@@ -127,17 +124,17 @@ let (check :
                                                      (Obj.magic
                                                         (FStar_Range.mk_range
                                                            "Pulse.Checker.WithLocalArray.fst"
-                                                           (Prims.of_int (63))
+                                                           (Prims.of_int (62))
                                                            (Prims.of_int (13))
-                                                           (Prims.of_int (63))
+                                                           (Prims.of_int (62))
                                                            (Prims.of_int (29)))))
                                                   (FStar_Sealed.seal
                                                      (Obj.magic
                                                         (FStar_Range.mk_range
                                                            "Pulse.Checker.WithLocalArray.fst"
-                                                           (Prims.of_int (64))
+                                                           (Prims.of_int (63))
                                                            (Prims.of_int (4))
-                                                           (Prims.of_int (79))
+                                                           (Prims.of_int (78))
                                                            (Prims.of_int (83)))))
                                                   (FStar_Tactics_Effect.lift_div_tac
                                                      (fun uu___1 ->
@@ -164,17 +161,17 @@ let (check :
                                                                     (Obj.magic
                                                                     (FStar_Range.mk_range
                                                                     "Pulse.Checker.WithLocalArray.fst"
-                                                                    (Prims.of_int (70))
+                                                                    (Prims.of_int (69))
                                                                     (Prims.of_int (10))
-                                                                    (Prims.of_int (71))
+                                                                    (Prims.of_int (70))
                                                                     (Prims.of_int (35)))))
                                                                     (FStar_Sealed.seal
                                                                     (Obj.magic
                                                                     (FStar_Range.mk_range
                                                                     "Pulse.Checker.WithLocalArray.fst"
-                                                                    (Prims.of_int (69))
+                                                                    (Prims.of_int (68))
                                                                     (Prims.of_int (8))
-                                                                    (Prims.of_int (71))
+                                                                    (Prims.of_int (70))
                                                                     (Prims.of_int (35)))))
                                                                     (Obj.magic
                                                                     (FStar_Tactics_Effect.tac_bind
@@ -182,9 +179,9 @@ let (check :
                                                                     (Obj.magic
                                                                     (FStar_Range.mk_range
                                                                     "Pulse.Checker.WithLocalArray.fst"
-                                                                    (Prims.of_int (71))
+                                                                    (Prims.of_int (70))
                                                                     (Prims.of_int (13))
-                                                                    (Prims.of_int (71))
+                                                                    (Prims.of_int (70))
                                                                     (Prims.of_int (34)))))
                                                                     (FStar_Sealed.seal
                                                                     (Obj.magic
@@ -225,17 +222,17 @@ let (check :
                                                                     (Obj.magic
                                                                     (FStar_Range.mk_range
                                                                     "Pulse.Checker.WithLocalArray.fst"
-                                                                    (Prims.of_int (73))
+                                                                    (Prims.of_int (72))
                                                                     (Prims.of_int (33))
-                                                                    (Prims.of_int (73))
+                                                                    (Prims.of_int (72))
                                                                     (Prims.of_int (52)))))
                                                                     (FStar_Sealed.seal
                                                                     (Obj.magic
                                                                     (FStar_Range.mk_range
                                                                     "Pulse.Checker.WithLocalArray.fst"
-                                                                    (Prims.of_int (72))
+                                                                    (Prims.of_int (71))
                                                                     (Prims.of_int (18))
-                                                                    (Prims.of_int (79))
+                                                                    (Prims.of_int (78))
                                                                     (Prims.of_int (83)))))
                                                                     (Obj.magic
                                                                     (Pulse_Checker_Pure.check_universe
@@ -257,17 +254,17 @@ let (check :
                                                                     (Obj.magic
                                                                     (FStar_Range.mk_range
                                                                     "Pulse.Checker.WithLocalArray.fst"
-                                                                    (Prims.of_int (75))
+                                                                    (Prims.of_int (74))
                                                                     (Prims.of_int (10))
-                                                                    (Prims.of_int (75))
+                                                                    (Prims.of_int (74))
                                                                     (Prims.of_int (77)))))
                                                                     (FStar_Sealed.seal
                                                                     (Obj.magic
                                                                     (FStar_Range.mk_range
                                                                     "Pulse.Checker.WithLocalArray.fst"
-                                                                    (Prims.of_int (73))
+                                                                    (Prims.of_int (72))
                                                                     (Prims.of_int (55))
-                                                                    (Prims.of_int (79))
+                                                                    (Prims.of_int (78))
                                                                     (Prims.of_int (83)))))
                                                                     (Obj.magic
                                                                     (Pulse_Checker_Pure.check_term_with_expected_type_and_effect
@@ -307,17 +304,17 @@ let (check :
                                                               (Obj.magic
                                                                  (FStar_Range.mk_range
                                                                     "Pulse.Checker.WithLocalArray.fst"
-                                                                    (Prims.of_int (83))
+                                                                    (Prims.of_int (82))
                                                                     (Prims.of_int (4))
-                                                                    (Prims.of_int (83))
+                                                                    (Prims.of_int (82))
                                                                     (Prims.of_int (53)))))
                                                            (FStar_Sealed.seal
                                                               (Obj.magic
                                                                  (FStar_Range.mk_range
                                                                     "Pulse.Checker.WithLocalArray.fst"
-                                                                    (Prims.of_int (81))
+                                                                    (Prims.of_int (80))
                                                                     (Prims.of_int (4))
-                                                                    (Prims.of_int (140))
+                                                                    (Prims.of_int (139))
                                                                     (Prims.of_int (38)))))
                                                            (Obj.magic
                                                               (Pulse_Checker_Pure.check_tot_term_with_expected_type
@@ -342,17 +339,17 @@ let (check :
                                                                     (Obj.magic
                                                                     (FStar_Range.mk_range
                                                                     "Pulse.Checker.WithLocalArray.fst"
-                                                                    (Prims.of_int (86))
+                                                                    (Prims.of_int (85))
                                                                     (Prims.of_int (12))
-                                                                    (Prims.of_int (86))
+                                                                    (Prims.of_int (85))
                                                                     (Prims.of_int (19)))))
                                                                     (FStar_Sealed.seal
                                                                     (Obj.magic
                                                                     (FStar_Range.mk_range
                                                                     "Pulse.Checker.WithLocalArray.fst"
-                                                                    (Prims.of_int (86))
+                                                                    (Prims.of_int (85))
                                                                     (Prims.of_int (22))
-                                                                    (Prims.of_int (135))
+                                                                    (Prims.of_int (134))
                                                                     (Prims.of_int (63)))))
                                                                     (FStar_Tactics_Effect.lift_div_tac
                                                                     (fun
@@ -368,17 +365,17 @@ let (check :
                                                                     (Obj.magic
                                                                     (FStar_Range.mk_range
                                                                     "Pulse.Checker.WithLocalArray.fst"
-                                                                    (Prims.of_int (87))
+                                                                    (Prims.of_int (86))
                                                                     (Prims.of_int (13))
-                                                                    (Prims.of_int (87))
+                                                                    (Prims.of_int (86))
                                                                     (Prims.of_int (36)))))
                                                                     (FStar_Sealed.seal
                                                                     (Obj.magic
                                                                     (FStar_Range.mk_range
                                                                     "Pulse.Checker.WithLocalArray.fst"
-                                                                    (Prims.of_int (88))
+                                                                    (Prims.of_int (87))
                                                                     (Prims.of_int (4))
-                                                                    (Prims.of_int (135))
+                                                                    (Prims.of_int (134))
                                                                     (Prims.of_int (63)))))
                                                                     (FStar_Tactics_Effect.lift_div_tac
                                                                     (fun
@@ -401,17 +398,17 @@ let (check :
                                                                     (Obj.magic
                                                                     (FStar_Range.mk_range
                                                                     "Pulse.Checker.WithLocalArray.fst"
-                                                                    (Prims.of_int (91))
+                                                                    (Prims.of_int (90))
                                                                     (Prims.of_int (14))
-                                                                    (Prims.of_int (92))
+                                                                    (Prims.of_int (91))
                                                                     (Prims.of_int (54)))))
                                                                     (FStar_Sealed.seal
                                                                     (Obj.magic
                                                                     (FStar_Range.mk_range
                                                                     "Pulse.Checker.WithLocalArray.fst"
-                                                                    (Prims.of_int (89))
+                                                                    (Prims.of_int (88))
                                                                     (Prims.of_int (9))
-                                                                    (Prims.of_int (92))
+                                                                    (Prims.of_int (91))
                                                                     (Prims.of_int (54)))))
                                                                     (Obj.magic
                                                                     (FStar_Tactics_Effect.tac_bind
@@ -419,9 +416,9 @@ let (check :
                                                                     (Obj.magic
                                                                     (FStar_Range.mk_range
                                                                     "Pulse.Checker.WithLocalArray.fst"
-                                                                    (Prims.of_int (92))
+                                                                    (Prims.of_int (91))
                                                                     (Prims.of_int (17))
-                                                                    (Prims.of_int (92))
+                                                                    (Prims.of_int (91))
                                                                     (Prims.of_int (53)))))
                                                                     (FStar_Sealed.seal
                                                                     (Obj.magic
@@ -462,17 +459,17 @@ let (check :
                                                                     (Obj.magic
                                                                     (FStar_Range.mk_range
                                                                     "Pulse.Checker.WithLocalArray.fst"
-                                                                    (Prims.of_int (94))
+                                                                    (Prims.of_int (93))
                                                                     (Prims.of_int (17))
-                                                                    (Prims.of_int (94))
+                                                                    (Prims.of_int (93))
                                                                     (Prims.of_int (32)))))
                                                                     (FStar_Sealed.seal
                                                                     (Obj.magic
                                                                     (FStar_Range.mk_range
                                                                     "Pulse.Checker.WithLocalArray.fst"
-                                                                    (Prims.of_int (94))
+                                                                    (Prims.of_int (93))
                                                                     (Prims.of_int (35))
-                                                                    (Prims.of_int (135))
+                                                                    (Prims.of_int (134))
                                                                     (Prims.of_int (63)))))
                                                                     (FStar_Tactics_Effect.lift_div_tac
                                                                     (fun
@@ -489,17 +486,17 @@ let (check :
                                                                     (Obj.magic
                                                                     (FStar_Range.mk_range
                                                                     "Pulse.Checker.WithLocalArray.fst"
-                                                                    (Prims.of_int (95))
+                                                                    (Prims.of_int (94))
                                                                     (Prims.of_int (23))
-                                                                    (Prims.of_int (95))
-                                                                    (Prims.of_int (82)))))
+                                                                    (Prims.of_int (94))
+                                                                    (Prims.of_int (78)))))
                                                                     (FStar_Sealed.seal
                                                                     (Obj.magic
                                                                     (FStar_Range.mk_range
                                                                     "Pulse.Checker.WithLocalArray.fst"
-                                                                    (Prims.of_int (95))
-                                                                    (Prims.of_int (85))
-                                                                    (Prims.of_int (135))
+                                                                    (Prims.of_int (94))
+                                                                    (Prims.of_int (81))
+                                                                    (Prims.of_int (134))
                                                                     (Prims.of_int (63)))))
                                                                     (FStar_Tactics_Effect.lift_div_tac
                                                                     (fun
@@ -508,8 +505,7 @@ let (check :
                                                                     g1 x
                                                                     binder.Pulse_Syntax_Base.binder_ppname
                                                                     (Pulse_Typing.mk_array
-                                                                    init_t
-                                                                    len)))
+                                                                    init_t)))
                                                                     (fun
                                                                     uu___4 ->
                                                                     (fun
@@ -521,17 +517,17 @@ let (check :
                                                                     (Obj.magic
                                                                     (FStar_Range.mk_range
                                                                     "Pulse.Checker.WithLocalArray.fst"
-                                                                    (Prims.of_int (96))
+                                                                    (Prims.of_int (95))
                                                                     (Prims.of_int (21))
-                                                                    (Prims.of_int (96))
+                                                                    (Prims.of_int (95))
                                                                     (Prims.of_int (75)))))
                                                                     (FStar_Sealed.seal
                                                                     (Obj.magic
                                                                     (FStar_Range.mk_range
                                                                     "Pulse.Checker.WithLocalArray.fst"
-                                                                    (Prims.of_int (96))
+                                                                    (Prims.of_int (95))
                                                                     (Prims.of_int (78))
-                                                                    (Prims.of_int (135))
+                                                                    (Prims.of_int (134))
                                                                     (Prims.of_int (63)))))
                                                                     (FStar_Tactics_Effect.lift_div_tac
                                                                     (fun
@@ -552,17 +548,17 @@ let (check :
                                                                     (Obj.magic
                                                                     (FStar_Range.mk_range
                                                                     "Pulse.Checker.WithLocalArray.fst"
-                                                                    (Prims.of_int (98))
+                                                                    (Prims.of_int (97))
                                                                     (Prims.of_int (8))
-                                                                    (Prims.of_int (98))
+                                                                    (Prims.of_int (97))
                                                                     (Prims.of_int (87)))))
                                                                     (FStar_Sealed.seal
                                                                     (Obj.magic
                                                                     (FStar_Range.mk_range
                                                                     "Pulse.Checker.WithLocalArray.fst"
-                                                                    (Prims.of_int (98))
+                                                                    (Prims.of_int (97))
                                                                     (Prims.of_int (90))
-                                                                    (Prims.of_int (135))
+                                                                    (Prims.of_int (134))
                                                                     (Prims.of_int (63)))))
                                                                     (FStar_Tactics_Effect.lift_div_tac
                                                                     (fun
@@ -579,17 +575,17 @@ let (check :
                                                                     (Obj.magic
                                                                     (FStar_Range.mk_range
                                                                     "Pulse.Checker.WithLocalArray.fst"
-                                                                    (Prims.of_int (102))
+                                                                    (Prims.of_int (101))
                                                                     (Prims.of_int (8))
-                                                                    (Prims.of_int (105))
+                                                                    (Prims.of_int (104))
                                                                     (Prims.of_int (92)))))
                                                                     (FStar_Sealed.seal
                                                                     (Obj.magic
                                                                     (FStar_Range.mk_range
                                                                     "Pulse.Checker.WithLocalArray.fst"
-                                                                    (Prims.of_int (107))
+                                                                    (Prims.of_int (106))
                                                                     (Prims.of_int (6))
-                                                                    (Prims.of_int (135))
+                                                                    (Prims.of_int (134))
                                                                     (Prims.of_int (63)))))
                                                                     (match post_hint
                                                                     with
@@ -633,25 +629,24 @@ let (check :
                                                                     (Obj.magic
                                                                     (FStar_Range.mk_range
                                                                     "Pulse.Checker.WithLocalArray.fst"
-                                                                    (Prims.of_int (111))
+                                                                    (Prims.of_int (110))
                                                                     (Prims.of_int (24))
-                                                                    (Prims.of_int (111))
-                                                                    (Prims.of_int (60)))))
+                                                                    (Prims.of_int (110))
+                                                                    (Prims.of_int (56)))))
                                                                     (FStar_Sealed.seal
                                                                     (Obj.magic
                                                                     (FStar_Range.mk_range
                                                                     "Pulse.Checker.WithLocalArray.fst"
-                                                                    (Prims.of_int (111))
-                                                                    (Prims.of_int (63))
-                                                                    (Prims.of_int (135))
+                                                                    (Prims.of_int (110))
+                                                                    (Prims.of_int (59))
+                                                                    (Prims.of_int (134))
                                                                     (Prims.of_int (63)))))
                                                                     (FStar_Tactics_Effect.lift_div_tac
                                                                     (fun
                                                                     uu___5 ->
                                                                     extend_post_hint
                                                                     g1 post
-                                                                    init_t
-                                                                    len x))
+                                                                    init_t x))
                                                                     (fun
                                                                     uu___5 ->
                                                                     (fun
@@ -663,17 +658,17 @@ let (check :
                                                                     (Obj.magic
                                                                     (FStar_Range.mk_range
                                                                     "Pulse.Checker.WithLocalArray.fst"
-                                                                    (Prims.of_int (112))
+                                                                    (Prims.of_int (111))
                                                                     (Prims.of_int (52))
-                                                                    (Prims.of_int (115))
+                                                                    (Prims.of_int (114))
                                                                     (Prims.of_int (55)))))
                                                                     (FStar_Sealed.seal
                                                                     (Obj.magic
                                                                     (FStar_Range.mk_range
                                                                     "Pulse.Checker.WithLocalArray.fst"
-                                                                    (Prims.of_int (111))
-                                                                    (Prims.of_int (63))
-                                                                    (Prims.of_int (135))
+                                                                    (Prims.of_int (110))
+                                                                    (Prims.of_int (59))
+                                                                    (Prims.of_int (134))
                                                                     (Prims.of_int (63)))))
                                                                     (Obj.magic
                                                                     (FStar_Tactics_Effect.tac_bind
@@ -681,17 +676,17 @@ let (check :
                                                                     (Obj.magic
                                                                     (FStar_Range.mk_range
                                                                     "Pulse.Checker.WithLocalArray.fst"
-                                                                    (Prims.of_int (114))
+                                                                    (Prims.of_int (113))
                                                                     (Prims.of_int (12))
-                                                                    (Prims.of_int (114))
+                                                                    (Prims.of_int (113))
                                                                     (Prims.of_int (117)))))
                                                                     (FStar_Sealed.seal
                                                                     (Obj.magic
                                                                     (FStar_Range.mk_range
                                                                     "Pulse.Checker.WithLocalArray.fst"
-                                                                    (Prims.of_int (115))
+                                                                    (Prims.of_int (114))
                                                                     (Prims.of_int (10))
-                                                                    (Prims.of_int (115))
+                                                                    (Prims.of_int (114))
                                                                     (Prims.of_int (55)))))
                                                                     (Obj.magic
                                                                     (check1
@@ -737,17 +732,17 @@ let (check :
                                                                     (Obj.magic
                                                                     (FStar_Range.mk_range
                                                                     "Pulse.Checker.WithLocalArray.fst"
-                                                                    (Prims.of_int (119))
+                                                                    (Prims.of_int (118))
                                                                     (Prims.of_int (15))
-                                                                    (Prims.of_int (120))
+                                                                    (Prims.of_int (119))
                                                                     (Prims.of_int (44)))))
                                                                     (FStar_Sealed.seal
                                                                     (Obj.magic
                                                                     (FStar_Range.mk_range
                                                                     "Pulse.Checker.WithLocalArray.fst"
-                                                                    (Prims.of_int (118))
+                                                                    (Prims.of_int (117))
                                                                     (Prims.of_int (13))
-                                                                    (Prims.of_int (120))
+                                                                    (Prims.of_int (119))
                                                                     (Prims.of_int (44)))))
                                                                     (Obj.magic
                                                                     (FStar_Tactics_Effect.tac_bind
@@ -755,9 +750,9 @@ let (check :
                                                                     (Obj.magic
                                                                     (FStar_Range.mk_range
                                                                     "Pulse.Checker.WithLocalArray.fst"
-                                                                    (Prims.of_int (120))
+                                                                    (Prims.of_int (119))
                                                                     (Prims.of_int (18))
-                                                                    (Prims.of_int (120))
+                                                                    (Prims.of_int (119))
                                                                     (Prims.of_int (43)))))
                                                                     (FStar_Sealed.seal
                                                                     (Obj.magic
@@ -798,17 +793,17 @@ let (check :
                                                                     (Obj.magic
                                                                     (FStar_Range.mk_range
                                                                     "Pulse.Checker.WithLocalArray.fst"
-                                                                    (Prims.of_int (122))
+                                                                    (Prims.of_int (121))
                                                                     (Prims.of_int (21))
-                                                                    (Prims.of_int (122))
+                                                                    (Prims.of_int (121))
                                                                     (Prims.of_int (48)))))
                                                                     (FStar_Sealed.seal
                                                                     (Obj.magic
                                                                     (FStar_Range.mk_range
                                                                     "Pulse.Checker.WithLocalArray.fst"
-                                                                    (Prims.of_int (123))
+                                                                    (Prims.of_int (122))
                                                                     (Prims.of_int (79))
-                                                                    (Prims.of_int (135))
+                                                                    (Prims.of_int (134))
                                                                     (Prims.of_int (63)))))
                                                                     (FStar_Tactics_Effect.lift_div_tac
                                                                     (fun
@@ -826,17 +821,17 @@ let (check :
                                                                     (Obj.magic
                                                                     (FStar_Range.mk_range
                                                                     "Pulse.Checker.WithLocalArray.fst"
-                                                                    (Prims.of_int (124))
+                                                                    (Prims.of_int (123))
                                                                     (Prims.of_int (18))
-                                                                    (Prims.of_int (124))
+                                                                    (Prims.of_int (123))
                                                                     (Prims.of_int (79)))))
                                                                     (FStar_Sealed.seal
                                                                     (Obj.magic
                                                                     (FStar_Range.mk_range
                                                                     "Pulse.Checker.WithLocalArray.fst"
-                                                                    (Prims.of_int (124))
+                                                                    (Prims.of_int (123))
                                                                     (Prims.of_int (82))
-                                                                    (Prims.of_int (135))
+                                                                    (Prims.of_int (134))
                                                                     (Prims.of_int (63)))))
                                                                     (FStar_Tactics_Effect.lift_div_tac
                                                                     (fun
@@ -866,17 +861,17 @@ let (check :
                                                                     (Obj.magic
                                                                     (FStar_Range.mk_range
                                                                     "Pulse.Checker.WithLocalArray.fst"
-                                                                    (Prims.of_int (125))
+                                                                    (Prims.of_int (124))
                                                                     (Prims.of_int (24))
-                                                                    (Prims.of_int (127))
+                                                                    (Prims.of_int (126))
                                                                     (Prims.of_int (100)))))
                                                                     (FStar_Sealed.seal
                                                                     (Obj.magic
                                                                     (FStar_Range.mk_range
                                                                     "Pulse.Checker.WithLocalArray.fst"
-                                                                    (Prims.of_int (128))
+                                                                    (Prims.of_int (127))
                                                                     (Prims.of_int (12))
-                                                                    (Prims.of_int (135))
+                                                                    (Prims.of_int (134))
                                                                     (Prims.of_int (63)))))
                                                                     (Obj.magic
                                                                     (FStar_Tactics_Effect.tac_bind
@@ -884,17 +879,17 @@ let (check :
                                                                     (Obj.magic
                                                                     (FStar_Range.mk_range
                                                                     "Pulse.Checker.WithLocalArray.fst"
-                                                                    (Prims.of_int (126))
+                                                                    (Prims.of_int (125))
                                                                     (Prims.of_int (34))
-                                                                    (Prims.of_int (126))
+                                                                    (Prims.of_int (125))
                                                                     (Prims.of_int (59)))))
                                                                     (FStar_Sealed.seal
                                                                     (Obj.magic
                                                                     (FStar_Range.mk_range
                                                                     "Pulse.Checker.WithLocalArray.fst"
-                                                                    (Prims.of_int (127))
+                                                                    (Prims.of_int (126))
                                                                     (Prims.of_int (12))
-                                                                    (Prims.of_int (127))
+                                                                    (Prims.of_int (126))
                                                                     (Prims.of_int (100)))))
                                                                     (FStar_Tactics_Effect.lift_div_tac
                                                                     (fun
@@ -922,17 +917,17 @@ let (check :
                                                                     (Obj.magic
                                                                     (FStar_Range.mk_range
                                                                     "Pulse.Checker.WithLocalArray.fst"
-                                                                    (Prims.of_int (129))
+                                                                    (Prims.of_int (128))
                                                                     (Prims.of_int (18))
-                                                                    (Prims.of_int (134))
+                                                                    (Prims.of_int (133))
                                                                     (Prims.of_int (23)))))
                                                                     (FStar_Sealed.seal
                                                                     (Obj.magic
                                                                     (FStar_Range.mk_range
                                                                     "Pulse.Checker.WithLocalArray.fst"
-                                                                    (Prims.of_int (135))
+                                                                    (Prims.of_int (134))
                                                                     (Prims.of_int (10))
-                                                                    (Prims.of_int (135))
+                                                                    (Prims.of_int (134))
                                                                     (Prims.of_int (63)))))
                                                                     (FStar_Tactics_Effect.lift_div_tac
                                                                     (fun
@@ -963,8 +958,7 @@ let (check :
                                                                     =
                                                                     (Pulse_Typing.as_binder
                                                                     (Pulse_Typing.mk_array
-                                                                    init_t
-                                                                    len));
+                                                                    init_t));
                                                                     Pulse_Syntax_Base.initializer2
                                                                     = init;
                                                                     Pulse_Syntax_Base.length
@@ -994,45 +988,45 @@ let (check :
                                                                     (Obj.magic
                                                                     (FStar_Range.mk_range
                                                                     "Pulse.Checker.WithLocalArray.fst"
-                                                                    (Prims.of_int (138))
+                                                                    (Prims.of_int (137))
                                                                     (Prims.of_int (9))
-                                                                    (Prims.of_int (140))
+                                                                    (Prims.of_int (139))
+                                                                    (Prims.of_int (38)))))
+                                                                    (FStar_Sealed.seal
+                                                                    (Obj.magic
+                                                                    (FStar_Range.mk_range
+                                                                    "Pulse.Checker.WithLocalArray.fst"
+                                                                    (Prims.of_int (136))
+                                                                    (Prims.of_int (7))
+                                                                    (Prims.of_int (139))
+                                                                    (Prims.of_int (38)))))
+                                                                    (Obj.magic
+                                                                    (FStar_Tactics_Effect.tac_bind
+                                                                    (FStar_Sealed.seal
+                                                                    (Obj.magic
+                                                                    (FStar_Range.mk_range
+                                                                    "Pulse.Checker.WithLocalArray.fst"
+                                                                    (Prims.of_int (137))
+                                                                    (Prims.of_int (9))
+                                                                    (Prims.of_int (139))
                                                                     (Prims.of_int (38)))))
                                                                     (FStar_Sealed.seal
                                                                     (Obj.magic
                                                                     (FStar_Range.mk_range
                                                                     "Pulse.Checker.WithLocalArray.fst"
                                                                     (Prims.of_int (137))
-                                                                    (Prims.of_int (7))
-                                                                    (Prims.of_int (140))
-                                                                    (Prims.of_int (38)))))
-                                                                    (Obj.magic
-                                                                    (FStar_Tactics_Effect.tac_bind
-                                                                    (FStar_Sealed.seal
-                                                                    (Obj.magic
-                                                                    (FStar_Range.mk_range
-                                                                    "Pulse.Checker.WithLocalArray.fst"
-                                                                    (Prims.of_int (138))
                                                                     (Prims.of_int (9))
-                                                                    (Prims.of_int (140))
-                                                                    (Prims.of_int (38)))))
-                                                                    (FStar_Sealed.seal
-                                                                    (Obj.magic
-                                                                    (FStar_Range.mk_range
-                                                                    "Pulse.Checker.WithLocalArray.fst"
-                                                                    (Prims.of_int (138))
-                                                                    (Prims.of_int (9))
-                                                                    (Prims.of_int (140))
-                                                                    (Prims.of_int (38)))))
-                                                                    (Obj.magic
-                                                                    (FStar_Tactics_Effect.tac_bind
-                                                                    (FStar_Sealed.seal
-                                                                    (Obj.magic
-                                                                    (FStar_Range.mk_range
-                                                                    "Pulse.Checker.WithLocalArray.fst"
                                                                     (Prims.of_int (139))
+                                                                    (Prims.of_int (38)))))
+                                                                    (Obj.magic
+                                                                    (FStar_Tactics_Effect.tac_bind
+                                                                    (FStar_Sealed.seal
+                                                                    (Obj.magic
+                                                                    (FStar_Range.mk_range
+                                                                    "Pulse.Checker.WithLocalArray.fst"
+                                                                    (Prims.of_int (138))
                                                                     (Prims.of_int (12))
-                                                                    (Prims.of_int (139))
+                                                                    (Prims.of_int (138))
                                                                     (Prims.of_int (35)))))
                                                                     (FStar_Sealed.seal
                                                                     (Obj.magic
